cp, support for with inv in ghost

pulse/src/ocaml/plugin/generated/Pulse_Checker_WithInv.ml
@@ -512,6 +512,35 @@ let (find_inv_post :
                                                                     ()))))))
                                                       uu___)))) uu___)))
                          uu___)
+let (atomic_or_ghost_with_inames_and_pre_post :
+  Pulse_Syntax_Base.comp ->
+    Pulse_Syntax_Base.term ->
+      Pulse_Syntax_Base.term ->
+        Pulse_Syntax_Base.term -> Pulse_Syntax_Base.comp)
+  =
+  fun c ->
+    fun inames ->
+      fun pre ->
+        fun post ->
+          match c with
+          | Pulse_Syntax_Base.C_STAtomic (uu___, obs, s) ->
+              Pulse_Syntax_Base.C_STAtomic
+                (inames, obs,
+                  {
+                    Pulse_Syntax_Base.u = (s.Pulse_Syntax_Base.u);
+                    Pulse_Syntax_Base.res = (s.Pulse_Syntax_Base.res);
+                    Pulse_Syntax_Base.pre = pre;
+                    Pulse_Syntax_Base.post = post
+                  })
+          | Pulse_Syntax_Base.C_STGhost (uu___, s) ->
+              Pulse_Syntax_Base.C_STGhost
+                (inames,
+                  {
+                    Pulse_Syntax_Base.u = (s.Pulse_Syntax_Base.u);
+                    Pulse_Syntax_Base.res = (s.Pulse_Syntax_Base.res);
+                    Pulse_Syntax_Base.pre = pre;
+                    Pulse_Syntax_Base.post = post
+                  })
 let (check :
   Pulse_Typing_Env.env ->
     Pulse_Syntax_Base.term ->
@@ -534,13 +563,13 @@ let (check :
                   (FStar_Sealed.seal
                      (Obj.magic
                         (FStar_Range.mk_range "Pulse.Checker.WithInv.fst"
-                           (Prims.of_int (278)) (Prims.of_int (47))
-                           (Prims.of_int (278)) (Prims.of_int (53)))))
+                           (Prims.of_int (287)) (Prims.of_int (47))
+                           (Prims.of_int (287)) (Prims.of_int (53)))))
                   (FStar_Sealed.seal
                      (Obj.magic
                         (FStar_Range.mk_range "Pulse.Checker.WithInv.fst"
-                           (Prims.of_int (278)) Prims.int_one
-                           (Prims.of_int (437)) (Prims.of_int (59)))))
+                           (Prims.of_int (287)) Prims.int_one
+                           (Prims.of_int (469)) (Prims.of_int (59)))))
                   (FStar_Tactics_Effect.lift_div_tac
                      (fun uu___ -> t.Pulse_Syntax_Base.term1))
                   (fun uu___ ->
@@ -557,17 +586,17 @@ let (check :
                                     (Obj.magic
                                        (FStar_Range.mk_range
                                           "Pulse.Checker.WithInv.fst"
-                                          (Prims.of_int (280))
+                                          (Prims.of_int (289))
                                           (Prims.of_int (4))
-                                          (Prims.of_int (291))
+                                          (Prims.of_int (300))
                                           (Prims.of_int (67)))))
                                  (FStar_Sealed.seal
                                     (Obj.magic
                                        (FStar_Range.mk_range
                                           "Pulse.Checker.WithInv.fst"
-                                          (Prims.of_int (293))
-                                          (Prims.of_int (2))
-                                          (Prims.of_int (437))
+                                          (Prims.of_int (308))
+                                          (Prims.of_int (8))
+                                          (Prims.of_int (469))
                                           (Prims.of_int (59)))))
                                  (match (returns_inv, post_hint) with
                                   | (FStar_Pervasives_Native.None,
@@ -596,17 +625,17 @@ let (check :
                                                  (Obj.magic
                                                     (FStar_Range.mk_range
                                                        "Pulse.Checker.WithInv.fst"
-                                                       (Prims.of_int (287))
+                                                       (Prims.of_int (296))
                                                        (Prims.of_int (8))
-                                                       (Prims.of_int (289))
+                                                       (Prims.of_int (298))
                                                        (Prims.of_int (60)))))
                                               (FStar_Sealed.seal
                                                  (Obj.magic
                                                     (FStar_Range.mk_range
                                                        "Pulse.Checker.WithInv.fst"
-                                                       (Prims.of_int (286))
+                                                       (Prims.of_int (295))
                                                        (Prims.of_int (6))
-                                                       (Prims.of_int (289))
+                                                       (Prims.of_int (298))
                                                        (Prims.of_int (60)))))
                                               (Obj.magic
                                                  (FStar_Tactics_Effect.tac_bind
@@ -614,17 +643,17 @@ let (check :
                                                        (Obj.magic
                                                           (FStar_Range.mk_range
                                                              "Pulse.Checker.WithInv.fst"
-                                                             (Prims.of_int (287))
+                                                             (Prims.of_int (296))
                                                              (Prims.of_int (8))
-                                                             (Prims.of_int (289))
+                                                             (Prims.of_int (298))
                                                              (Prims.of_int (60)))))
                                                     (FStar_Sealed.seal
                                                        (Obj.magic
                                                           (FStar_Range.mk_range
                                                              "Pulse.Checker.WithInv.fst"
-                                                             (Prims.of_int (287))
+                                                             (Prims.of_int (296))
                                                              (Prims.of_int (8))
-                                                             (Prims.of_int (289))
+                                                             (Prims.of_int (298))
                                                              (Prims.of_int (60)))))
                                                     (Obj.magic
                                                        (FStar_Tactics_Effect.tac_bind
@@ -632,17 +661,17 @@ let (check :
                                                              (Obj.magic
                                                                 (FStar_Range.mk_range
                                                                    "Pulse.Checker.WithInv.fst"
-                                                                   (Prims.of_int (288))
+                                                                   (Prims.of_int (297))
                                                                    (Prims.of_int (10))
-                                                                   (Prims.of_int (288))
+                                                                   (Prims.of_int (297))
                                                                    (Prims.of_int (57)))))
                                                           (FStar_Sealed.seal
                                                              (Obj.magic
                                                                 (FStar_Range.mk_range
                                                                    "Pulse.Checker.WithInv.fst"
-                                                                   (Prims.of_int (287))
+                                                                   (Prims.of_int (296))
                                                                    (Prims.of_int (8))
-                                                                   (Prims.of_int (289))
+                                                                   (Prims.of_int (298))
                                                                    (Prims.of_int (60)))))
                                                           (Obj.magic
                                                              (FStar_Tactics_Effect.tac_bind
@@ -650,17 +679,17 @@ let (check :
                                                                    (Obj.magic
                                                                     (FStar_Range.mk_range
                                                                     "Pulse.Checker.WithInv.fst"
-                                                                    (Prims.of_int (288))
+                                                                    (Prims.of_int (297))
                                                                     (Prims.of_int (51))
-                                                                    (Prims.of_int (288))
+                                                                    (Prims.of_int (297))
                                                                     (Prims.of_int (57)))))
                                                                 (FStar_Sealed.seal
                                                                    (Obj.magic
                                                                     (FStar_Range.mk_range
                                                                     "Pulse.Checker.WithInv.fst"
-                                                                    (Prims.of_int (288))
+                                                                    (Prims.of_int (297))
                                                                     (Prims.of_int (10))
-                                                                    (Prims.of_int (288))
+                                                                    (Prims.of_int (297))
                                                                     (Prims.of_int (57)))))
                                                                 (Obj.magic
                                                                    (Pulse_PP.pp
@@ -685,17 +714,17 @@ let (check :
                                                                     (Obj.magic
                                                                     (FStar_Range.mk_range
                                                                     "Pulse.Checker.WithInv.fst"
-                                                                    (Prims.of_int (287))
+                                                                    (Prims.of_int (296))
                                                                     (Prims.of_int (8))
-                                                                    (Prims.of_int (289))
+                                                                    (Prims.of_int (298))
                                                                     (Prims.of_int (60)))))
                                                                     (FStar_Sealed.seal
                                                                     (Obj.magic
                                                                     (FStar_Range.mk_range
                                                                     "Pulse.Checker.WithInv.fst"
-                                                                    (Prims.of_int (287))
+                                                                    (Prims.of_int (296))
                                                                     (Prims.of_int (8))
-                                                                    (Prims.of_int (289))
+                                                                    (Prims.of_int (298))
                                                                     (Prims.of_int (60)))))
                                                                     (Obj.magic
                                                                     (FStar_Tactics_Effect.tac_bind
@@ -703,17 +732,17 @@ let (check :
                                                                     (Obj.magic
                                                                     (FStar_Range.mk_range
                                                                     "Pulse.Checker.WithInv.fst"
-                                                                    (Prims.of_int (289))
+                                                                    (Prims.of_int (298))
                                                                     (Prims.of_int (10))
-                                                                    (Prims.of_int (289))
+                                                                    (Prims.of_int (298))
                                                                     (Prims.of_int (58)))))
                                                                     (FStar_Sealed.seal
                                                                     (Obj.magic
                                                                     (FStar_Range.mk_range
                                                                     "Pulse.Checker.WithInv.fst"
-                                                                    (Prims.of_int (287))
+                                                                    (Prims.of_int (296))
                                                                     (Prims.of_int (8))
-                                                                    (Prims.of_int (289))
+                                                                    (Prims.of_int (298))
                                                                     (Prims.of_int (60)))))
                                                                     (Obj.magic
                                                                     (FStar_Tactics_Effect.tac_bind
@@ -721,17 +750,17 @@ let (check :
                                                                     (Obj.magic
                                                                     (FStar_Range.mk_range
                                                                     "Pulse.Checker.WithInv.fst"
-                                                                    (Prims.of_int (289))
+                                                                    (Prims.of_int (298))
                                                                     (Prims.of_int (52))
-                                                                    (Prims.of_int (289))
+                                                                    (Prims.of_int (298))
                                                                     (Prims.of_int (58)))))
                                                                     (FStar_Sealed.seal
                                                                     (Obj.magic
                                                                     (FStar_Range.mk_range
                                                                     "Pulse.Checker.WithInv.fst"
-                                                                    (Prims.of_int (289))
+                                                                    (Prims.of_int (298))
                                                                     (Prims.of_int (10))
-                                                                    (Prims.of_int (289))
+                                                                    (Prims.of_int (298))
                                                                     (Prims.of_int (58)))))
                                                                     (Obj.magic
                                                                     (Pulse_PP.pp
@@ -785,90 +814,79 @@ let (check :
                                               "Fatal: no post hint on with_invariant")))
                                  (fun uu___1 ->
                                     (fun post_hint1 ->
-                                       match post_hint1.Pulse_Typing.effect_annot
-                                       with
-                                       | Pulse_Syntax_Base.EffectAnnotGhost
-                                           uu___1 ->
-                                           Obj.magic
-                                             (Pulse_Typing_Env.fail_doc g
-                                                (FStar_Pervasives_Native.Some
-                                                   (t.Pulse_Syntax_Base.range1))
-                                                [FStar_Pprint.doc_of_string
-                                                   "Cannot open invariants in a 'ghost' context"])
-                                       | uu___1 ->
-                                           Obj.magic
-                                             (FStar_Tactics_Effect.tac_bind
-                                                (FStar_Sealed.seal
-                                                   (Obj.magic
-                                                      (FStar_Range.mk_range
-                                                         "Pulse.Checker.WithInv.fst"
-                                                         (Prims.of_int (302))
-                                                         (Prims.of_int (21))
-                                                         (Prims.of_int (302))
-                                                         (Prims.of_int (31)))))
-                                                (FStar_Sealed.seal
-                                                   (Obj.magic
-                                                      (FStar_Range.mk_range
-                                                         "Pulse.Checker.WithInv.fst"
-                                                         (Prims.of_int (302))
-                                                         (Prims.of_int (34))
-                                                         (Prims.of_int (437))
-                                                         (Prims.of_int (59)))))
-                                                (FStar_Tactics_Effect.lift_div_tac
-                                                   (fun uu___2 ->
-                                                      body.Pulse_Syntax_Base.range1))
-                                                (fun uu___2 ->
-                                                   (fun body_range ->
-                                                      Obj.magic
-                                                        (FStar_Tactics_Effect.tac_bind
-                                                           (FStar_Sealed.seal
-                                                              (Obj.magic
-                                                                 (FStar_Range.mk_range
-                                                                    "Pulse.Checker.WithInv.fst"
-                                                                    (Prims.of_int (303))
-                                                                    (Prims.of_int (18))
-                                                                    (Prims.of_int (303))
-                                                                    (Prims.of_int (52)))))
-                                                           (FStar_Sealed.seal
-                                                              (Obj.magic
-                                                                 (FStar_Range.mk_range
-                                                                    "Pulse.Checker.WithInv.fst"
-                                                                    (Prims.of_int (303))
-                                                                    (Prims.of_int (55))
-                                                                    (Prims.of_int (437))
-                                                                    (Prims.of_int (59)))))
-                                                           (FStar_Tactics_Effect.lift_div_tac
-                                                              (fun uu___2 ->
-                                                                 Pulse_RuntimeUtils.range_of_term
-                                                                   i))
-                                                           (fun uu___2 ->
-                                                              (fun i_range ->
-                                                                 Obj.magic
-                                                                   (FStar_Tactics_Effect.tac_bind
-                                                                    (FStar_Sealed.seal
+                                       Obj.magic
+                                         (FStar_Tactics_Effect.tac_bind
+                                            (FStar_Sealed.seal
+                                               (Obj.magic
+                                                  (FStar_Range.mk_range
+                                                     "Pulse.Checker.WithInv.fst"
+                                                     (Prims.of_int (311))
+                                                     (Prims.of_int (21))
+                                                     (Prims.of_int (311))
+                                                     (Prims.of_int (31)))))
+                                            (FStar_Sealed.seal
+                                               (Obj.magic
+                                                  (FStar_Range.mk_range
+                                                     "Pulse.Checker.WithInv.fst"
+                                                     (Prims.of_int (311))
+                                                     (Prims.of_int (34))
+                                                     (Prims.of_int (469))
+                                                     (Prims.of_int (59)))))
+                                            (FStar_Tactics_Effect.lift_div_tac
+                                               (fun uu___1 ->
+                                                  body.Pulse_Syntax_Base.range1))
+                                            (fun uu___1 ->
+                                               (fun body_range ->
+                                                  Obj.magic
+                                                    (FStar_Tactics_Effect.tac_bind
+                                                       (FStar_Sealed.seal
+                                                          (Obj.magic
+                                                             (FStar_Range.mk_range
+                                                                "Pulse.Checker.WithInv.fst"
+                                                                (Prims.of_int (312))
+                                                                (Prims.of_int (18))
+                                                                (Prims.of_int (312))
+                                                                (Prims.of_int (52)))))
+                                                       (FStar_Sealed.seal
+                                                          (Obj.magic
+                                                             (FStar_Range.mk_range
+                                                                "Pulse.Checker.WithInv.fst"
+                                                                (Prims.of_int (312))
+                                                                (Prims.of_int (55))
+                                                                (Prims.of_int (469))
+                                                                (Prims.of_int (59)))))
+                                                       (FStar_Tactics_Effect.lift_div_tac
+                                                          (fun uu___1 ->
+                                                             Pulse_RuntimeUtils.range_of_term
+                                                               i))
+                                                       (fun uu___1 ->
+                                                          (fun i_range ->
+                                                             Obj.magic
+                                                               (FStar_Tactics_Effect.tac_bind
+                                                                  (FStar_Sealed.seal
                                                                     (Obj.magic
                                                                     (FStar_Range.mk_range
                                                                     "Pulse.Checker.WithInv.fst"
-                                                                    (Prims.of_int (305))
+                                                                    (Prims.of_int (314))
                                                                     (Prims.of_int (14))
-                                                                    (Prims.of_int (305))
+                                                                    (Prims.of_int (314))
                                                                     (Prims.of_int (35)))))
-                                                                    (FStar_Sealed.seal
+                                                                  (FStar_Sealed.seal
                                                                     (Obj.magic
                                                                     (FStar_Range.mk_range
                                                                     "Pulse.Checker.WithInv.fst"
-                                                                    (Prims.of_int (306))
+                                                                    (Prims.of_int (315))
                                                                     (Prims.of_int (4))
-                                                                    (Prims.of_int (437))
+                                                                    (Prims.of_int (469))
                                                                     (Prims.of_int (59)))))
-                                                                    (FStar_Tactics_Effect.lift_div_tac
+                                                                  (FStar_Tactics_Effect.lift_div_tac
                                                                     (fun
-                                                                    uu___2 ->
+                                                                    uu___1 ->
                                                                     find_inv
                                                                     g pre ()
                                                                     i))
-                                                                    (fun
-                                                                    uu___2 ->
+                                                                  (fun uu___1
+                                                                    ->
                                                                     (fun res
                                                                     ->
                                                                     Obj.magic
@@ -877,17 +895,17 @@ let (check :
                                                                     (Obj.magic
                                                                     (FStar_Range.mk_range
                                                                     "Pulse.Checker.WithInv.fst"
-                                                                    (Prims.of_int (306))
+                                                                    (Prims.of_int (315))
                                                                     (Prims.of_int (4))
-                                                                    (Prims.of_int (306))
+                                                                    (Prims.of_int (315))
                                                                     (Prims.of_int (76)))))
                                                                     (FStar_Sealed.seal
                                                                     (Obj.magic
                                                                     (FStar_Range.mk_range
                                                                     "Pulse.Checker.WithInv.fst"
-                                                                    (Prims.of_int (306))
+                                                                    (Prims.of_int (315))
                                                                     (Prims.of_int (77))
-                                                                    (Prims.of_int (437))
+                                                                    (Prims.of_int (469))
                                                                     (Prims.of_int (59)))))
                                                                     (if
                                                                     FStar_Pervasives_Native.uu___is_None
@@ -905,39 +923,39 @@ let (check :
                                                                     (Obj.repr
                                                                     (FStar_Tactics_Effect.lift_div_tac
                                                                     (fun
-                                                                    uu___3 ->
+                                                                    uu___2 ->
                                                                     ()))))
                                                                     (fun
-                                                                    uu___2 ->
+                                                                    uu___1 ->
                                                                     (fun
-                                                                    uu___2 ->
+                                                                    uu___1 ->
                                                                     Obj.magic
                                                                     (FStar_Tactics_Effect.tac_bind
                                                                     (FStar_Sealed.seal
                                                                     (Obj.magic
                                                                     (FStar_Range.mk_range
                                                                     "Pulse.Checker.WithInv.fst"
-                                                                    (Prims.of_int (308))
+                                                                    (Prims.of_int (317))
                                                                     (Prims.of_int (80))
-                                                                    (Prims.of_int (308))
+                                                                    (Prims.of_int (317))
                                                                     (Prims.of_int (83)))))
                                                                     (FStar_Sealed.seal
                                                                     (Obj.magic
                                                                     (FStar_Range.mk_range
                                                                     "Pulse.Checker.WithInv.fst"
-                                                                    (Prims.of_int (306))
+                                                                    (Prims.of_int (315))
                                                                     (Prims.of_int (77))
-                                                                    (Prims.of_int (437))
+                                                                    (Prims.of_int (469))
                                                                     (Prims.of_int (59)))))
                                                                     (FStar_Tactics_Effect.lift_div_tac
                                                                     (fun
-                                                                    uu___3 ->
+                                                                    uu___2 ->
                                                                     res))
                                                                     (fun
-                                                                    uu___3 ->
+                                                                    uu___2 ->
                                                                     (fun
-                                                                    uu___3 ->
-                                                                    match uu___3
+                                                                    uu___2 ->
+                                                                    match uu___2
                                                                     with
                                                                     | 
                                                                     FStar_Pervasives_Native.Some
@@ -954,26 +972,26 @@ let (check :
                                                                     (Obj.magic
                                                                     (FStar_Range.mk_range
                                                                     "Pulse.Checker.WithInv.fst"
-                                                                    (Prims.of_int (310))
+                                                                    (Prims.of_int (319))
                                                                     (Prims.of_int (27))
-                                                                    (Prims.of_int (310))
+                                                                    (Prims.of_int (319))
                                                                     (Prims.of_int (46)))))
                                                                     (FStar_Sealed.seal
                                                                     (Obj.magic
                                                                     (FStar_Range.mk_range
                                                                     "Pulse.Checker.WithInv.fst"
-                                                                    (Prims.of_int (310))
+                                                                    (Prims.of_int (319))
                                                                     (Prims.of_int (49))
-                                                                    (Prims.of_int (437))
+                                                                    (Prims.of_int (469))
                                                                     (Prims.of_int (59)))))
                                                                     (FStar_Tactics_Effect.lift_div_tac
                                                                     (fun
-                                                                    uu___4 ->
+                                                                    uu___3 ->
                                                                     Pulse_Syntax_Pure.tm_star
                                                                     p
                                                                     pre_frame))
                                                                     (fun
-                                                                    uu___4 ->
+                                                                    uu___3 ->
                                                                     (fun
                                                                     pre_body
                                                                     ->
@@ -983,24 +1001,24 @@ let (check :
                                                                     (Obj.magic
                                                                     (FStar_Range.mk_range
                                                                     "Pulse.Checker.WithInv.fst"
-                                                                    (Prims.of_int (317))
+                                                                    (Prims.of_int (326))
                                                                     (Prims.of_int (59))
-                                                                    (Prims.of_int (317))
+                                                                    (Prims.of_int (326))
                                                                     (Prims.of_int (67)))))
                                                                     (FStar_Sealed.seal
                                                                     (Obj.magic
                                                                     (FStar_Range.mk_range
                                                                     "Pulse.Checker.WithInv.fst"
-                                                                    (Prims.of_int (317))
+                                                                    (Prims.of_int (326))
                                                                     (Prims.of_int (70))
-                                                                    (Prims.of_int (437))
+                                                                    (Prims.of_int (469))
                                                                     (Prims.of_int (59)))))
                                                                     (FStar_Tactics_Effect.lift_div_tac
                                                                     (fun
-                                                                    uu___4 ->
+                                                                    uu___3 ->
                                                                     ()))
                                                                     (fun
-                                                                    uu___4 ->
+                                                                    uu___3 ->
                                                                     (fun
                                                                     pre_body_typing
                                                                     ->
@@ -1010,25 +1028,25 @@ let (check :
                                                                     (Obj.magic
                                                                     (FStar_Range.mk_range
                                                                     "Pulse.Checker.WithInv.fst"
-                                                                    (Prims.of_int (319))
+                                                                    (Prims.of_int (328))
                                                                     (Prims.of_int (12))
-                                                                    (Prims.of_int (319))
+                                                                    (Prims.of_int (328))
                                                                     (Prims.of_int (19)))))
                                                                     (FStar_Sealed.seal
                                                                     (Obj.magic
                                                                     (FStar_Range.mk_range
                                                                     "Pulse.Checker.WithInv.fst"
-                                                                    (Prims.of_int (320))
+                                                                    (Prims.of_int (329))
                                                                     (Prims.of_int (53))
-                                                                    (Prims.of_int (437))
+                                                                    (Prims.of_int (469))
                                                                     (Prims.of_int (59)))))
                                                                     (FStar_Tactics_Effect.lift_div_tac
                                                                     (fun
-                                                                    uu___4 ->
+                                                                    uu___3 ->
                                                                     Pulse_Typing_Env.fresh
                                                                     g))
                                                                     (fun
-                                                                    uu___4 ->
+                                                                    uu___3 ->
                                                                     (fun x ->
                                                                     Obj.magic
                                                                     (FStar_Tactics_Effect.tac_bind
@@ -1036,27 +1054,27 @@ let (check :
                                                                     (Obj.magic
                                                                     (FStar_Range.mk_range
                                                                     "Pulse.Checker.WithInv.fst"
-                                                                    (Prims.of_int (321))
+                                                                    (Prims.of_int (330))
                                                                     (Prims.of_int (13))
-                                                                    (Prims.of_int (321))
+                                                                    (Prims.of_int (330))
                                                                     (Prims.of_int (63)))))
                                                                     (FStar_Sealed.seal
                                                                     (Obj.magic
                                                                     (FStar_Range.mk_range
                                                                     "Pulse.Checker.WithInv.fst"
-                                                                    (Prims.of_int (321))
+                                                                    (Prims.of_int (330))
                                                                     (Prims.of_int (66))
-                                                                    (Prims.of_int (437))
+                                                                    (Prims.of_int (469))
                                                                     (Prims.of_int (59)))))
                                                                     (FStar_Tactics_Effect.lift_div_tac
                                                                     (fun
-                                                                    uu___4 ->
+                                                                    uu___3 ->
                                                                     Pulse_Typing_Env.push_binding
                                                                     g x
                                                                     Pulse_Syntax_Base.ppname_default
                                                                     post_hint1.Pulse_Typing.ret_ty))
                                                                     (fun
-                                                                    uu___4 ->
+                                                                    uu___3 ->
                                                                     (fun g'
                                                                     ->
                                                                     Obj.magic
@@ -1065,17 +1083,17 @@ let (check :
                                                                     (Obj.magic
                                                                     (FStar_Range.mk_range
                                                                     "Pulse.Checker.WithInv.fst"
-                                                                    (Prims.of_int (323))
+                                                                    (Prims.of_int (332))
                                                                     (Prims.of_int (53))
-                                                                    (Prims.of_int (323))
+                                                                    (Prims.of_int (332))
                                                                     (Prims.of_int (63)))))
                                                                     (FStar_Sealed.seal
                                                                     (Obj.magic
                                                                     (FStar_Range.mk_range
                                                                     "Pulse.Checker.WithInv.fst"
-                                                                    (Prims.of_int (323))
+                                                                    (Prims.of_int (332))
                                                                     (Prims.of_int (66))
-                                                                    (Prims.of_int (437))
+                                                                    (Prims.of_int (469))
                                                                     (Prims.of_int (59)))))
                                                                     (Obj.magic
                                                                     (recheck
@@ -1085,7 +1103,7 @@ let (check :
                                                                     post_hint1.Pulse_Typing.u)
                                                                     ()))
                                                                     (fun
-                                                                    uu___4 ->
+                                                                    uu___3 ->
                                                                     (fun
                                                                     post_hint_ret_ty_typing
                                                                     ->
@@ -1095,17 +1113,17 @@ let (check :
                                                                     (Obj.magic
                                                                     (FStar_Range.mk_range
                                                                     "Pulse.Checker.WithInv.fst"
-                                                                    (Prims.of_int (328))
+                                                                    (Prims.of_int (337))
                                                                     (Prims.of_int (8))
-                                                                    (Prims.of_int (328))
+                                                                    (Prims.of_int (337))
                                                                     (Prims.of_int (18)))))
                                                                     (FStar_Sealed.seal
                                                                     (Obj.magic
                                                                     (FStar_Range.mk_range
                                                                     "Pulse.Checker.WithInv.fst"
-                                                                    (Prims.of_int (329))
+                                                                    (Prims.of_int (338))
                                                                     (Prims.of_int (6))
-                                                                    (Prims.of_int (437))
+                                                                    (Prims.of_int (469))
                                                                     (Prims.of_int (59)))))
                                                                     (Obj.magic
                                                                     (recheck
@@ -1117,7 +1135,7 @@ let (check :
                                                                     Pulse_Syntax_Pure.tm_vprop
                                                                     ()))
                                                                     (fun
-                                                                    uu___4 ->
+                                                                    uu___3 ->
                                                                     (fun
                                                                     post_hint_post_typing
                                                                     ->
@@ -1127,17 +1145,17 @@ let (check :
                                                                     (Obj.magic
                                                                     (FStar_Range.mk_range
                                                                     "Pulse.Checker.WithInv.fst"
-                                                                    (Prims.of_int (331))
+                                                                    (Prims.of_int (340))
                                                                     (Prims.of_int (14))
-                                                                    (Prims.of_int (338))
+                                                                    (Prims.of_int (347))
                                                                     (Prims.of_int (7)))))
                                                                     (FStar_Sealed.seal
                                                                     (Obj.magic
                                                                     (FStar_Range.mk_range
                                                                     "Pulse.Checker.WithInv.fst"
-                                                                    (Prims.of_int (340))
+                                                                    (Prims.of_int (349))
                                                                     (Prims.of_int (4))
-                                                                    (Prims.of_int (437))
+                                                                    (Prims.of_int (469))
                                                                     (Prims.of_int (59)))))
                                                                     (Obj.magic
                                                                     (find_inv_post
@@ -1147,7 +1165,7 @@ let (check :
                                                                     post_hint1.Pulse_Typing.post
                                                                     () () i))
                                                                     (fun
-                                                                    uu___4 ->
+                                                                    uu___3 ->
                                                                     (fun res1
                                                                     ->
                                                                     Obj.magic
@@ -1156,17 +1174,17 @@ let (check :
                                                                     (Obj.magic
                                                                     (FStar_Range.mk_range
                                                                     "Pulse.Checker.WithInv.fst"
-                                                                    (Prims.of_int (340))
+                                                                    (Prims.of_int (349))
                                                                     (Prims.of_int (4))
-                                                                    (Prims.of_int (340))
+                                                                    (Prims.of_int (349))
                                                                     (Prims.of_int (82)))))
                                                                     (FStar_Sealed.seal
                                                                     (Obj.magic
                                                                     (FStar_Range.mk_range
                                                                     "Pulse.Checker.WithInv.fst"
-                                                                    (Prims.of_int (340))
+                                                                    (Prims.of_int (349))
                                                                     (Prims.of_int (83))
-                                                                    (Prims.of_int (437))
+                                                                    (Prims.of_int (469))
                                                                     (Prims.of_int (59)))))
                                                                     (if
                                                                     FStar_Pervasives_Native.uu___is_None
@@ -1184,46 +1202,46 @@ let (check :
                                                                     (Obj.repr
                                                                     (FStar_Tactics_Effect.lift_div_tac
                                                                     (fun
-                                                                    uu___5 ->
+                                                                    uu___4 ->
                                                                     ()))))
                                                                     (fun
-                                                                    uu___4 ->
+                                                                    uu___3 ->
                                                                     (fun
-                                                                    uu___4 ->
+                                                                    uu___3 ->
                                                                     Obj.magic
                                                                     (FStar_Tactics_Effect.tac_bind
                                                                     (FStar_Sealed.seal
                                                                     (Obj.magic
                                                                     (FStar_Range.mk_range
                                                                     "Pulse.Checker.WithInv.fst"
-                                                                    (Prims.of_int (342))
+                                                                    (Prims.of_int (351))
                                                                     (Prims.of_int (78))
-                                                                    (Prims.of_int (342))
+                                                                    (Prims.of_int (351))
                                                                     (Prims.of_int (81)))))
                                                                     (FStar_Sealed.seal
                                                                     (Obj.magic
                                                                     (FStar_Range.mk_range
                                                                     "Pulse.Checker.WithInv.fst"
-                                                                    (Prims.of_int (340))
+                                                                    (Prims.of_int (349))
                                                                     (Prims.of_int (83))
-                                                                    (Prims.of_int (437))
+                                                                    (Prims.of_int (469))
                                                                     (Prims.of_int (59)))))
                                                                     (FStar_Tactics_Effect.lift_div_tac
                                                                     (fun
-                                                                    uu___5 ->
+                                                                    uu___4 ->
                                                                     res1))
                                                                     (fun
-                                                                    uu___5 ->
+                                                                    uu___4 ->
                                                                     (fun
-                                                                    uu___5 ->
-                                                                    match uu___5
+                                                                    uu___4 ->
+                                                                    match uu___4
                                                                     with
                                                                     | 
                                                                     FStar_Pervasives_Native.Some
                                                                     (FStar_Pervasives.Mkdtuple5
                                                                     (p',
                                                                     post_frame,
-                                                                    uu___6,
+                                                                    uu___5,
                                                                     post_frame_typing,
                                                                     d_post_frame_equiv))
                                                                     ->
@@ -1233,26 +1251,26 @@ let (check :
                                                                     (Obj.magic
                                                                     (FStar_Range.mk_range
                                                                     "Pulse.Checker.WithInv.fst"
-                                                                    (Prims.of_int (345))
+                                                                    (Prims.of_int (354))
                                                                     (Prims.of_int (20))
-                                                                    (Prims.of_int (345))
+                                                                    (Prims.of_int (354))
                                                                     (Prims.of_int (40)))))
                                                                     (FStar_Sealed.seal
                                                                     (Obj.magic
                                                                     (FStar_Range.mk_range
                                                                     "Pulse.Checker.WithInv.fst"
-                                                                    (Prims.of_int (345))
+                                                                    (Prims.of_int (354))
                                                                     (Prims.of_int (43))
-                                                                    (Prims.of_int (437))
+                                                                    (Prims.of_int (469))
                                                                     (Prims.of_int (59)))))
                                                                     (FStar_Tactics_Effect.lift_div_tac
                                                                     (fun
-                                                                    uu___7 ->
+                                                                    uu___6 ->
                                                                     Pulse_Syntax_Pure.tm_star
                                                                     p
                                                                     post_frame))
                                                                     (fun
-                                                                    uu___7 ->
+                                                                    uu___6 ->
                                                                     (fun
                                                                     post_body
                                                                     ->
@@ -1262,21 +1280,21 @@ let (check :
                                                                     (Obj.magic
                                                                     (FStar_Range.mk_range
                                                                     "Pulse.Checker.WithInv.fst"
-                                                                    (Prims.of_int (349))
+                                                                    (Prims.of_int (358))
                                                                     (Prims.of_int (8))
-                                                                    (Prims.of_int (353))
+                                                                    (Prims.of_int (363))
                                                                     (Prims.of_int (75)))))
                                                                     (FStar_Sealed.seal
                                                                     (Obj.magic
                                                                     (FStar_Range.mk_range
                                                                     "Pulse.Checker.WithInv.fst"
-                                                                    (Prims.of_int (345))
+                                                                    (Prims.of_int (354))
                                                                     (Prims.of_int (43))
-                                                                    (Prims.of_int (437))
+                                                                    (Prims.of_int (469))
                                                                     (Prims.of_int (59)))))
                                                                     (FStar_Tactics_Effect.lift_div_tac
                                                                     (fun
-                                                                    uu___7 ->
+                                                                    uu___6 ->
                                                                     match 
                                                                     post_hint1.Pulse_Typing.effect_annot
                                                                     with
@@ -1285,6 +1303,15 @@ let (check :
                                                                     ->
                                                                     Prims.Mkdtuple2
                                                                     (all_inames,
+                                                                    ())
+                                                                    | 
+                                                                    Pulse_Syntax_Base.EffectAnnotGhost
+                                                                    {
+                                                                    Pulse_Syntax_Base.opens
+                                                                    = opens;_}
+                                                                    ->
+                                                                    Prims.Mkdtuple2
+                                                                    (opens,
                                                                     ())
                                                                     | 
                                                                     Pulse_Syntax_Base.EffectAnnotAtomic
@@ -1296,10 +1323,10 @@ let (check :
                                                                     (opens,
                                                                     ())))
                                                                     (fun
-                                                                    uu___7 ->
+                                                                    uu___6 ->
                                                                     (fun
-                                                                    uu___7 ->
-                                                                    match uu___7
+                                                                    uu___6 ->
+                                                                    match uu___6
                                                                     with
                                                                     | 
                                                                     Prims.Mkdtuple2
@@ -1312,51 +1339,51 @@ let (check :
                                                                     (Obj.magic
                                                                     (FStar_Range.mk_range
                                                                     "Pulse.Checker.WithInv.fst"
-                                                                    (Prims.of_int (354))
+                                                                    (Prims.of_int (364))
                                                                     (Prims.of_int (6))
-                                                                    (Prims.of_int (437))
+                                                                    (Prims.of_int (469))
                                                                     (Prims.of_int (59)))))
                                                                     (FStar_Sealed.seal
                                                                     (Obj.magic
                                                                     (FStar_Range.mk_range
                                                                     "Pulse.Checker.WithInv.fst"
-                                                                    (Prims.of_int (354))
+                                                                    (Prims.of_int (364))
                                                                     (Prims.of_int (6))
-                                                                    (Prims.of_int (437))
+                                                                    (Prims.of_int (469))
                                                                     (Prims.of_int (59)))))
                                                                     (FStar_Tactics_Effect.lift_div_tac
                                                                     (fun
-                                                                    uu___8 ->
-                                                                    uu___7))
+                                                                    uu___7 ->
+                                                                    uu___6))
                                                                     (fun
-                                                                    uu___8 ->
+                                                                    uu___7 ->
                                                                     (fun
-                                                                    uu___8 ->
+                                                                    uu___7 ->
                                                                     Obj.magic
                                                                     (FStar_Tactics_Effect.tac_bind
                                                                     (FStar_Sealed.seal
                                                                     (Obj.magic
                                                                     (FStar_Range.mk_range
                                                                     "Pulse.Checker.WithInv.fst"
-                                                                    (Prims.of_int (355))
+                                                                    (Prims.of_int (365))
                                                                     (Prims.of_int (25))
-                                                                    (Prims.of_int (355))
+                                                                    (Prims.of_int (365))
                                                                     (Prims.of_int (45)))))
                                                                     (FStar_Sealed.seal
                                                                     (Obj.magic
                                                                     (FStar_Range.mk_range
                                                                     "Pulse.Checker.WithInv.fst"
-                                                                    (Prims.of_int (355))
+                                                                    (Prims.of_int (365))
                                                                     (Prims.of_int (48))
-                                                                    (Prims.of_int (437))
+                                                                    (Prims.of_int (469))
                                                                     (Prims.of_int (59)))))
                                                                     (FStar_Tactics_Effect.lift_div_tac
                                                                     (fun
-                                                                    uu___9 ->
+                                                                    uu___8 ->
                                                                     remove_iname
                                                                     opens i))
                                                                     (fun
-                                                                    uu___9 ->
+                                                                    uu___8 ->
                                                                     (fun
                                                                     opens_remove_i
                                                                     ->
@@ -1366,29 +1393,53 @@ let (check :
                                                                     (Obj.magic
                                                                     (FStar_Range.mk_range
                                                                     "Pulse.Checker.WithInv.fst"
-                                                                    (Prims.of_int (356))
-                                                                    (Prims.of_int (23))
-                                                                    (Prims.of_int (356))
-                                                                    (Prims.of_int (65)))))
+                                                                    (Prims.of_int (367))
+                                                                    (Prims.of_int (6))
+                                                                    (Prims.of_int (372))
+                                                                    (Prims.of_int (49)))))
                                                                     (FStar_Sealed.seal
                                                                     (Obj.magic
                                                                     (FStar_Range.mk_range
                                                                     "Pulse.Checker.WithInv.fst"
-                                                                    (Prims.of_int (356))
-                                                                    (Prims.of_int (68))
-                                                                    (Prims.of_int (437))
+                                                                    (Prims.of_int (372))
+                                                                    (Prims.of_int (52))
+                                                                    (Prims.of_int (469))
                                                                     (Prims.of_int (59)))))
                                                                     (FStar_Tactics_Effect.lift_div_tac
                                                                     (fun
+                                                                    uu___8 ->
+                                                                    match 
+                                                                    post_hint1.Pulse_Typing.effect_annot
+                                                                    with
+                                                                    | 
+                                                                    Pulse_Syntax_Base.EffectAnnotSTT
+                                                                    ->
+                                                                    Pulse_Syntax_Base.EffectAnnotAtomic
+                                                                    {
+                                                                    Pulse_Syntax_Base.opens1
+                                                                    =
+                                                                    opens_remove_i
+                                                                    }
+                                                                    | 
+                                                                    Pulse_Syntax_Base.EffectAnnotAtomic
                                                                     uu___9 ->
                                                                     Pulse_Syntax_Base.EffectAnnotAtomic
                                                                     {
                                                                     Pulse_Syntax_Base.opens1
                                                                     =
                                                                     opens_remove_i
+                                                                    }
+                                                                    | 
+                                                                    Pulse_Syntax_Base.EffectAnnotGhost
+                                                                    uu___9 ->
+                                                                    Pulse_Syntax_Base.EffectAnnotGhost
+                                                                    {
+                                                                    Pulse_Syntax_Base.opens
+                                                                    =
+                                                                    opens_remove_i
                                                                     }))
                                                                     (fun
-                                                                    uu___9 ->
+                                                                    uu___8 ->
                                                                     (fun
                                                                     effect_annot
                                                                     ->
@@ -1398,28 +1449,28 @@ let (check :
                                                                     (Obj.magic
                                                                     (FStar_Range.mk_range
                                                                     "Pulse.Checker.WithInv.fst"
-                                                                    (Prims.of_int (359))
+                                                                    (Prims.of_int (375))
                                                                     (Prims.of_int (8))
-                                                                    (Prims.of_int (359))
+                                                                    (Prims.of_int (375))
                                                                     (Prims.of_int (63)))))
                                                                     (FStar_Sealed.seal
                                                                     (Obj.magic
                                                                     (FStar_Range.mk_range
                                                                     "Pulse.Checker.WithInv.fst"
-                                                                    (Prims.of_int (362))
+                                                                    (Prims.of_int (378))
                                                                     (Prims.of_int (48))
-                                                                    (Prims.of_int (437))
+                                                                    (Prims.of_int (469))
                                                                     (Prims.of_int (59)))))
                                                                     (FStar_Tactics_Effect.lift_div_tac
                                                                     (fun
-                                                                    uu___9 ->
+                                                                    uu___8 ->
                                                                     (fun
-                                                                    uu___9 ->
+                                                                    uu___8 ->
                                                                     Obj.magic
                                                                     ())
-                                                                    uu___9))
+                                                                    uu___8))
                                                                     (fun
-                                                                    uu___9 ->
+                                                                    uu___8 ->
                                                                     (fun
                                                                     effect_annot_typing
                                                                     ->
@@ -1429,21 +1480,21 @@ let (check :
                                                                     (Obj.magic
                                                                     (FStar_Range.mk_range
                                                                     "Pulse.Checker.WithInv.fst"
-                                                                    (Prims.of_int (363))
+                                                                    (Prims.of_int (379))
                                                                     (Prims.of_int (50))
-                                                                    (Prims.of_int (371))
+                                                                    (Prims.of_int (387))
                                                                     (Prims.of_int (27)))))
                                                                     (FStar_Sealed.seal
                                                                     (Obj.magic
                                                                     (FStar_Range.mk_range
                                                                     "Pulse.Checker.WithInv.fst"
-                                                                    (Prims.of_int (372))
+                                                                    (Prims.of_int (388))
                                                                     (Prims.of_int (8))
-                                                                    (Prims.of_int (437))
+                                                                    (Prims.of_int (469))
                                                                     (Prims.of_int (59)))))
                                                                     (FStar_Tactics_Effect.lift_div_tac
                                                                     (fun
-                                                                    uu___9 ->
+                                                                    uu___8 ->
                                                                     {
                                                                     Pulse_Typing.g
                                                                     = g;
@@ -1472,7 +1523,7 @@ let (check :
                                                                     = ()
                                                                     }))
                                                                     (fun
-                                                                    uu___9 ->
+                                                                    uu___8 ->
                                                                     (fun
                                                                     post_hint_body
                                                                     ->
@@ -1482,17 +1533,17 @@ let (check :
                                                                     (Obj.magic
                                                                     (FStar_Range.mk_range
                                                                     "Pulse.Checker.WithInv.fst"
-                                                                    (Prims.of_int (374))
+                                                                    (Prims.of_int (390))
                                                                     (Prims.of_int (41))
-                                                                    (Prims.of_int (377))
+                                                                    (Prims.of_int (393))
                                                                     (Prims.of_int (37)))))
                                                                     (FStar_Sealed.seal
                                                                     (Obj.magic
                                                                     (FStar_Range.mk_range
                                                                     "Pulse.Checker.WithInv.fst"
-                                                                    (Prims.of_int (372))
+                                                                    (Prims.of_int (388))
                                                                     (Prims.of_int (8))
-                                                                    (Prims.of_int (437))
+                                                                    (Prims.of_int (469))
                                                                     (Prims.of_int (59)))))
                                                                     (Obj.magic
                                                                     (FStar_Tactics_Effect.tac_bind
@@ -1500,25 +1551,25 @@ let (check :
                                                                     (Obj.magic
                                                                     (FStar_Range.mk_range
                                                                     "Pulse.Checker.WithInv.fst"
-                                                                    (Prims.of_int (375))
+                                                                    (Prims.of_int (391))
                                                                     (Prims.of_int (19))
-                                                                    (Prims.of_int (375))
+                                                                    (Prims.of_int (391))
                                                                     (Prims.of_int (53)))))
                                                                     (FStar_Sealed.seal
                                                                     (Obj.magic
                                                                     (FStar_Range.mk_range
                                                                     "Pulse.Checker.WithInv.fst"
-                                                                    (Prims.of_int (375))
+                                                                    (Prims.of_int (391))
                                                                     (Prims.of_int (56))
-                                                                    (Prims.of_int (377))
+                                                                    (Prims.of_int (393))
                                                                     (Prims.of_int (37)))))
                                                                     (FStar_Tactics_Effect.lift_div_tac
                                                                     (fun
-                                                                    uu___9 ->
+                                                                    uu___8 ->
                                                                     Pulse_Syntax_Base.mk_ppname_no_range
                                                                     "with_inv_body"))
                                                                     (fun
-                                                                    uu___9 ->
+                                                                    uu___8 ->
                                                                     (fun
                                                                     ppname ->
                                                                     Obj.magic
@@ -1527,17 +1578,17 @@ let (check :
                                                                     (Obj.magic
                                                                     (FStar_Range.mk_range
                                                                     "Pulse.Checker.WithInv.fst"
-                                                                    (Prims.of_int (376))
+                                                                    (Prims.of_int (392))
                                                                     (Prims.of_int (14))
-                                                                    (Prims.of_int (376))
+                                                                    (Prims.of_int (392))
                                                                     (Prims.of_int (80)))))
                                                                     (FStar_Sealed.seal
                                                                     (Obj.magic
                                                                     (FStar_Range.mk_range
                                                                     "Pulse.Checker.WithInv.fst"
-                                                                    (Prims.of_int (377))
+                                                                    (Prims.of_int (393))
                                                                     (Prims.of_int (6))
-                                                                    (Prims.of_int (377))
+                                                                    (Prims.of_int (393))
                                                                     (Prims.of_int (37)))))
                                                                     (Obj.magic
                                                                     (check1 g
@@ -1548,7 +1599,7 @@ let (check :
                                                                     ppname
                                                                     body))
                                                                     (fun
-                                                                    uu___9 ->
+                                                                    uu___8 ->
                                                                     (fun r ->
                                                                     Obj.magic
                                                                     (Pulse_Checker_Base.apply_checker_result_k
@@ -1556,13 +1607,13 @@ let (check :
                                                                     pre_body
                                                                     post_hint_body
                                                                     r ppname))
-                                                                    uu___9)))
-                                                                    uu___9)))
+                                                                    uu___8)))
+                                                                    uu___8)))
                                                                     (fun
-                                                                    uu___9 ->
+                                                                    uu___8 ->
                                                                     (fun
-                                                                    uu___9 ->
-                                                                    match uu___9
+                                                                    uu___8 ->
+                                                                    match uu___8
                                                                     with
                                                                     | 
                                                                     FStar_Pervasives.Mkdtuple3
@@ -1576,77 +1627,30 @@ let (check :
                                                                     (Obj.magic
                                                                     (FStar_Range.mk_range
                                                                     "Pulse.Checker.WithInv.fst"
-                                                                    (Prims.of_int (380))
-                                                                    (Prims.of_int (35))
-                                                                    (Prims.of_int (380))
-                                                                    (Prims.of_int (41)))))
-                                                                    (FStar_Sealed.seal
-                                                                    (Obj.magic
-                                                                    (FStar_Range.mk_range
-                                                                    "Pulse.Checker.WithInv.fst"
-                                                                    (Prims.of_int (378))
-                                                                    (Prims.of_int (6))
-                                                                    (Prims.of_int (437))
-                                                                    (Prims.of_int (59)))))
-                                                                    (FStar_Tactics_Effect.lift_div_tac
-                                                                    (fun
-                                                                    uu___10
-                                                                    -> c_body))
-                                                                    (fun
-                                                                    uu___10
-                                                                    ->
-                                                                    (fun
-                                                                    uu___10
-                                                                    ->
-                                                                    match uu___10
-                                                                    with
-                                                                    | 
-                                                                    Pulse_Syntax_Base.C_STAtomic
-                                                                    (inames,
-                                                                    obs, st)
-                                                                    ->
-                                                                    Obj.magic
-                                                                    (FStar_Tactics_Effect.tac_bind
-                                                                    (FStar_Sealed.seal
-                                                                    (Obj.magic
-                                                                    (FStar_Range.mk_range
-                                                                    "Pulse.Checker.WithInv.fst"
-                                                                    (Prims.of_int (385))
+                                                                    (Prims.of_int (400))
                                                                     (Prims.of_int (16))
-                                                                    (Prims.of_int (387))
-                                                                    (Prims.of_int (29)))))
+                                                                    (Prims.of_int (403))
+                                                                    (Prims.of_int (20)))))
                                                                     (FStar_Sealed.seal
                                                                     (Obj.magic
                                                                     (FStar_Range.mk_range
                                                                     "Pulse.Checker.WithInv.fst"
-                                                                    (Prims.of_int (387))
-                                                                    (Prims.of_int (32))
-                                                                    (Prims.of_int (437))
+                                                                    (Prims.of_int (403))
+                                                                    (Prims.of_int (23))
+                                                                    (Prims.of_int (469))
                                                                     (Prims.of_int (59)))))
                                                                     (FStar_Tactics_Effect.lift_div_tac
                                                                     (fun
-                                                                    uu___11
-                                                                    ->
-                                                                    Pulse_Syntax_Base.C_STAtomic
-                                                                    ((Pulse_Reflection_Util.add_inv_tm
-                                                                    inames i),
-                                                                    obs,
-                                                                    {
-                                                                    Pulse_Syntax_Base.u
-                                                                    =
-                                                                    (st.Pulse_Syntax_Base.u);
-                                                                    Pulse_Syntax_Base.res
-                                                                    =
-                                                                    (st.Pulse_Syntax_Base.res);
-                                                                    Pulse_Syntax_Base.pre
-                                                                    = pre;
-                                                                    Pulse_Syntax_Base.post
-                                                                    =
-                                                                    (post_hint1.Pulse_Typing.post)
-                                                                    })))
+                                                                    uu___9 ->
+                                                                    atomic_or_ghost_with_inames_and_pre_post
+                                                                    c_body
+                                                                    (Pulse_Reflection_Util.add_inv_tm
+                                                                    (Pulse_Syntax_Base.comp_inames
+                                                                    c_body) i)
+                                                                    pre
+                                                                    post_hint1.Pulse_Typing.post))
                                                                     (fun
-                                                                    uu___11
-                                                                    ->
+                                                                    uu___9 ->
                                                                     (fun
                                                                     c_out ->
                                                                     Obj.magic
@@ -1655,24 +1659,23 @@ let (check :
                                                                     (Obj.magic
                                                                     (FStar_Range.mk_range
                                                                     "Pulse.Checker.WithInv.fst"
-                                                                    (Prims.of_int (389))
+                                                                    (Prims.of_int (405))
                                                                     (Prims.of_int (14))
-                                                                    (Prims.of_int (389))
+                                                                    (Prims.of_int (405))
                                                                     (Prims.of_int (47)))))
                                                                     (FStar_Sealed.seal
                                                                     (Obj.magic
                                                                     (FStar_Range.mk_range
                                                                     "Pulse.Checker.WithInv.fst"
-                                                                    (Prims.of_int (389))
+                                                                    (Prims.of_int (405))
                                                                     (Prims.of_int (50))
-                                                                    (Prims.of_int (437))
+                                                                    (Prims.of_int (469))
                                                                     (Prims.of_int (59)))))
                                                                     (Obj.magic
                                                                     (disjointness_remove_i_i
                                                                     g opens i))
                                                                     (fun
-                                                                    uu___11
-                                                                    ->
+                                                                    uu___9 ->
                                                                     (fun tok
                                                                     ->
                                                                     Obj.magic
@@ -1681,27 +1684,71 @@ let (check :
                                                                     (Obj.magic
                                                                     (FStar_Range.mk_range
                                                                     "Pulse.Checker.WithInv.fst"
-                                                                    (Prims.of_int (390))
-                                                                    (Prims.of_int (33))
-                                                                    (Prims.of_int (419))
-                                                                    (Prims.of_int (52)))))
+                                                                    (Prims.of_int (407))
+                                                                    (Prims.of_int (13))
+                                                                    (Prims.of_int (407))
+                                                                    (Prims.of_int (92)))))
                                                                     (FStar_Sealed.seal
                                                                     (Obj.magic
                                                                     (FStar_Range.mk_range
                                                                     "Pulse.Checker.WithInv.fst"
-                                                                    (Prims.of_int (422))
-                                                                    (Prims.of_int (4))
-                                                                    (Prims.of_int (437))
+                                                                    (Prims.of_int (407))
+                                                                    (Prims.of_int (95))
+                                                                    (Prims.of_int (469))
                                                                     (Prims.of_int (59)))))
                                                                     (FStar_Tactics_Effect.lift_div_tac
                                                                     (fun
-                                                                    uu___11
+                                                                    uu___9 ->
+                                                                    Pulse_Typing.wtag
+                                                                    (FStar_Pervasives_Native.Some
+                                                                    (Pulse_Syntax_Base.ctag_of_comp_st
+                                                                    c_out))
+                                                                    (Pulse_Syntax_Base.Tm_WithInv
+                                                                    {
+                                                                    Pulse_Syntax_Base.name1
+                                                                    = i;
+                                                                    Pulse_Syntax_Base.body6
+                                                                    = body1;
+                                                                    Pulse_Syntax_Base.returns_inv
+                                                                    =
+                                                                    FStar_Pervasives_Native.None
+                                                                    })))
+                                                                    (fun
+                                                                    uu___9 ->
+                                                                    (fun tm
                                                                     ->
+                                                                    Obj.magic
+                                                                    (FStar_Tactics_Effect.tac_bind
+                                                                    (FStar_Sealed.seal
+                                                                    (Obj.magic
+                                                                    (FStar_Range.mk_range
+                                                                    "Pulse.Checker.WithInv.fst"
+                                                                    (Prims.of_int (408))
+                                                                    (Prims.of_int (34))
+                                                                    (Prims.of_int (447))
+                                                                    (Prims.of_int (7)))))
+                                                                    (FStar_Sealed.seal
+                                                                    (Obj.magic
+                                                                    (FStar_Range.mk_range
+                                                                    "Pulse.Checker.WithInv.fst"
+                                                                    (Prims.of_int (449))
+                                                                    (Prims.of_int (4))
+                                                                    (Prims.of_int (469))
+                                                                    (Prims.of_int (59)))))
+                                                                    (FStar_Tactics_Effect.lift_div_tac
+                                                                    (fun
+                                                                    uu___9 ->
                                                                     Pulse_Typing.T_Equiv
                                                                     (g,
                                                                     (Pulse_Typing.wtag
                                                                     (FStar_Pervasives_Native.Some
-                                                                    Pulse_Syntax_Base.STT_Atomic)
+                                                                    (Pulse_Syntax_Base.ctag_of_comp_st
+                                                                    (atomic_or_ghost_with_inames_and_pre_post
+                                                                    c_body
+                                                                    (Pulse_Syntax_Base.comp_inames
+                                                                    c_body)
+                                                                    pre_frame
+                                                                    post_frame)))
                                                                     (Pulse_Syntax_Base.Tm_WithInv
                                                                     {
                                                                     Pulse_Syntax_Base.name1
@@ -1712,80 +1759,47 @@ let (check :
                                                                     =
                                                                     FStar_Pervasives_Native.None
                                                                     })),
-                                                                    (Pulse_Syntax_Base.C_STAtomic
-                                                                    ((Pulse_Reflection_Util.add_inv_tm
-                                                                    inames i),
-                                                                    obs,
-                                                                    {
-                                                                    Pulse_Syntax_Base.u
-                                                                    =
-                                                                    (st.Pulse_Syntax_Base.u);
-                                                                    Pulse_Syntax_Base.res
-                                                                    =
-                                                                    (st.Pulse_Syntax_Base.res);
-                                                                    Pulse_Syntax_Base.pre
-                                                                    =
+                                                                    (atomic_or_ghost_with_inames_and_pre_post
+                                                                    c_body
+                                                                    (Pulse_Reflection_Util.add_inv_tm
+                                                                    (Pulse_Syntax_Base.comp_inames
+                                                                    c_body) i)
                                                                     (Pulse_Syntax_Pure.tm_star
                                                                     (Pulse_Syntax_Pure.tm_inv
                                                                     i p)
-                                                                    pre_frame);
-                                                                    Pulse_Syntax_Base.post
-                                                                    =
+                                                                    pre_frame)
                                                                     (Pulse_Syntax_Pure.tm_star
                                                                     (Pulse_Syntax_Pure.tm_inv
                                                                     i p)
-                                                                    post_frame)
-                                                                    })),
+                                                                    post_frame)),
                                                                     c_out,
                                                                     (Pulse_Typing.T_WithInv
                                                                     (g, i, p,
                                                                     body1,
-                                                                    (Pulse_Syntax_Base.C_STAtomic
-                                                                    (inames,
-                                                                    obs,
-                                                                    {
-                                                                    Pulse_Syntax_Base.u
-                                                                    =
-                                                                    (st.Pulse_Syntax_Base.u);
-                                                                    Pulse_Syntax_Base.res
-                                                                    =
-                                                                    (st.Pulse_Syntax_Base.res);
-                                                                    Pulse_Syntax_Base.pre
-                                                                    =
-                                                                    pre_frame;
-                                                                    Pulse_Syntax_Base.post
-                                                                    =
-                                                                    post_frame
-                                                                    })), (),
-                                                                    (),
+                                                                    (atomic_or_ghost_with_inames_and_pre_post
+                                                                    c_body
+                                                                    (Pulse_Syntax_Base.comp_inames
+                                                                    c_body)
+                                                                    pre_frame
+                                                                    post_frame),
+                                                                    (), (),
                                                                     body_typing,
                                                                     ())),
                                                                     (Pulse_Typing.ST_VPropEquiv
                                                                     (g,
-                                                                    (Pulse_Syntax_Base.C_STAtomic
-                                                                    ((Pulse_Reflection_Util.add_inv_tm
-                                                                    inames i),
-                                                                    obs,
-                                                                    {
-                                                                    Pulse_Syntax_Base.u
-                                                                    =
-                                                                    (st.Pulse_Syntax_Base.u);
-                                                                    Pulse_Syntax_Base.res
-                                                                    =
-                                                                    (st.Pulse_Syntax_Base.res);
-                                                                    Pulse_Syntax_Base.pre
-                                                                    =
+                                                                    (atomic_or_ghost_with_inames_and_pre_post
+                                                                    c_body
+                                                                    (Pulse_Reflection_Util.add_inv_tm
+                                                                    (Pulse_Syntax_Base.comp_inames
+                                                                    c_body) i)
                                                                     (Pulse_Syntax_Pure.tm_star
                                                                     (Pulse_Syntax_Pure.tm_inv
                                                                     i p)
-                                                                    pre_frame);
-                                                                    Pulse_Syntax_Base.post
-                                                                    =
+                                                                    pre_frame)
                                                                     (Pulse_Syntax_Pure.tm_star
                                                                     (Pulse_Syntax_Pure.tm_inv
                                                                     i p)
-                                                                    post_frame)
-                                                                    })),
+                                                                    post_frame)),
                                                                     c_out, x,
                                                                     (), (),
                                                                     (),
@@ -1794,102 +1808,54 @@ let (check :
                                                                     g),
                                                                     (Pulse_Elaborate_Pure.elab_term
                                                                     (Pulse_Syntax_Base.comp_res
-                                                                    (Pulse_Syntax_Base.C_STAtomic
-                                                                    ((Pulse_Reflection_Util.add_inv_tm
-                                                                    inames i),
-                                                                    obs,
-                                                                    {
-                                                                    Pulse_Syntax_Base.u
-                                                                    =
-                                                                    (st.Pulse_Syntax_Base.u);
-                                                                    Pulse_Syntax_Base.res
-                                                                    =
-                                                                    (st.Pulse_Syntax_Base.res);
-                                                                    Pulse_Syntax_Base.pre
-                                                                    =
+                                                                    (atomic_or_ghost_with_inames_and_pre_post
+                                                                    c_body
+                                                                    (Pulse_Reflection_Util.add_inv_tm
+                                                                    (Pulse_Syntax_Base.comp_inames
+                                                                    c_body) i)
                                                                     (Pulse_Syntax_Pure.tm_star
                                                                     (Pulse_Syntax_Pure.tm_inv
                                                                     i p)
-                                                                    pre_frame);
-                                                                    Pulse_Syntax_Base.post
-                                                                    =
+                                                                    pre_frame)
                                                                     (Pulse_Syntax_Pure.tm_star
                                                                     (Pulse_Syntax_Pure.tm_inv
                                                                     i p)
-                                                                    post_frame)
-                                                                    })))),
+                                                                    post_frame)))),
                                                                     FStar_Reflection_Typing.R_Eq)),
                                                                     (), ())))))
                                                                     (fun
-                                                                    uu___11
-                                                                    ->
+                                                                    uu___9 ->
                                                                     (fun d ->
                                                                     match 
                                                                     post_hint1.Pulse_Typing.effect_annot
                                                                     with
                                                                     | 
-                                                                    Pulse_Syntax_Base.EffectAnnotAtomic
-                                                                    uu___11
-                                                                    ->
+                                                                    Pulse_Syntax_Base.EffectAnnotGhost
+                                                                    uu___9 ->
                                                                     Obj.magic
                                                                     (FStar_Tactics_Effect.tac_bind
                                                                     (FStar_Sealed.seal
                                                                     (Obj.magic
                                                                     (FStar_Range.mk_range
                                                                     "Pulse.Checker.WithInv.fst"
-                                                                    (Prims.of_int (424))
-                                                                    (Prims.of_int (38))
-                                                                    (Prims.of_int (424))
-                                                                    (Prims.of_int (43)))))
-                                                                    (FStar_Sealed.seal
-                                                                    (Obj.magic
-                                                                    (FStar_Range.mk_range
-                                                                    "Pulse.Checker.WithInv.fst"
-                                                                    (Prims.of_int (423))
-                                                                    (Prims.of_int (28))
-                                                                    (Prims.of_int (433))
-                                                                    (Prims.of_int (59)))))
-                                                                    (FStar_Tactics_Effect.lift_div_tac
-                                                                    (fun
-                                                                    uu___12
-                                                                    -> c_out))
-                                                                    (fun
-                                                                    uu___12
-                                                                    ->
-                                                                    (fun
-                                                                    uu___12
-                                                                    ->
-                                                                    match uu___12
-                                                                    with
-                                                                    | 
-                                                                    Pulse_Syntax_Base.C_STAtomic
-                                                                    (add_inv,
-                                                                    obs1,
-                                                                    st1) ->
-                                                                    Obj.magic
-                                                                    (FStar_Tactics_Effect.tac_bind
-                                                                    (FStar_Sealed.seal
-                                                                    (Obj.magic
-                                                                    (FStar_Range.mk_range
-                                                                    "Pulse.Checker.WithInv.fst"
-                                                                    (Prims.of_int (426))
+                                                                    (Prims.of_int (453))
                                                                     (Prims.of_int (8))
-                                                                    (Prims.of_int (428))
-                                                                    (Prims.of_int (22)))))
+                                                                    (Prims.of_int (453))
+                                                                    (Prims.of_int (60)))))
                                                                     (FStar_Sealed.seal
                                                                     (Obj.magic
                                                                     (FStar_Range.mk_range
                                                                     "Pulse.Checker.WithInv.fst"
-                                                                    (Prims.of_int (429))
+                                                                    (Prims.of_int (454))
                                                                     (Prims.of_int (8))
-                                                                    (Prims.of_int (433))
+                                                                    (Prims.of_int (465))
                                                                     (Prims.of_int (59)))))
                                                                     (Obj.magic
                                                                     (add_remove_inverse
                                                                     g opens i
                                                                     () ()))
                                                                     (fun
-                                                                    uu___13
+                                                                    uu___10
                                                                     ->
                                                                     (fun tok1
                                                                     ->
@@ -1899,81 +1865,124 @@ let (check :
                                                                     (Obj.magic
                                                                     (FStar_Range.mk_range
                                                                     "Pulse.Checker.WithInv.fst"
-                                                                    (Prims.of_int (430))
-                                                                    (Prims.of_int (18))
-                                                                    (Prims.of_int (430))
-                                                                    (Prims.of_int (41)))))
+                                                                    (Prims.of_int (456))
+                                                                    (Prims.of_int (8))
+                                                                    (Prims.of_int (462))
+                                                                    (Prims.of_int (51)))))
                                                                     (FStar_Sealed.seal
                                                                     (Obj.magic
                                                                     (FStar_Range.mk_range
                                                                     "Pulse.Checker.WithInv.fst"
-                                                                    (Prims.of_int (430))
-                                                                    (Prims.of_int (44))
-                                                                    (Prims.of_int (433))
+                                                                    (Prims.of_int (454))
+                                                                    (Prims.of_int (8))
+                                                                    (Prims.of_int (465))
                                                                     (Prims.of_int (59)))))
                                                                     (FStar_Tactics_Effect.lift_div_tac
                                                                     (fun
-                                                                    uu___13
+                                                                    uu___10
                                                                     ->
+                                                                    match c_out
+                                                                    with
+                                                                    | 
                                                                     Pulse_Syntax_Base.C_STAtomic
+                                                                    (add_inv,
+                                                                    obs, st)
+                                                                    ->
+                                                                    Prims.Mkdtuple2
+                                                                    ((Pulse_Syntax_Base.C_STAtomic
                                                                     (opens,
-                                                                    obs1,
-                                                                    st1)))
+                                                                    obs, st)),
+                                                                    (Pulse_Typing.STS_AtomicInvs
+                                                                    (g, st,
+                                                                    add_inv,
+                                                                    opens,
+                                                                    obs, obs,
+                                                                    ())))
+                                                                    | 
+                                                                    Pulse_Syntax_Base.C_STGhost
+                                                                    (add_inv,
+                                                                    st) ->
+                                                                    Prims.Mkdtuple2
+                                                                    ((Pulse_Syntax_Base.C_STGhost
+                                                                    (opens,
+                                                                    st)),
+                                                                    (Pulse_Typing.STS_GhostInvs
+                                                                    (g, st,
+                                                                    add_inv,
+                                                                    opens,
+                                                                    ())))))
                                                                     (fun
-                                                                    uu___13
+                                                                    uu___10
                                                                     ->
                                                                     (fun
-                                                                    c_out1 ->
+                                                                    uu___10
+                                                                    ->
+                                                                    match uu___10
+                                                                    with
+                                                                    | 
+                                                                    Prims.Mkdtuple2
+                                                                    (c_out_opens,
+                                                                    d_sub_c)
+                                                                    ->
                                                                     Obj.magic
                                                                     (FStar_Tactics_Effect.tac_bind
                                                                     (FStar_Sealed.seal
                                                                     (Obj.magic
                                                                     (FStar_Range.mk_range
                                                                     "Pulse.Checker.WithInv.fst"
-                                                                    (Prims.of_int (432))
-                                                                    (Prims.of_int (8))
-                                                                    (Prims.of_int (432))
-                                                                    (Prims.of_int (71)))))
+                                                                    (Prims.of_int (462))
+                                                                    (Prims.of_int (54))
+                                                                    (Prims.of_int (465))
+                                                                    (Prims.of_int (59)))))
                                                                     (FStar_Sealed.seal
                                                                     (Obj.magic
                                                                     (FStar_Range.mk_range
                                                                     "Pulse.Checker.WithInv.fst"
-                                                                    (Prims.of_int (433))
-                                                                    (Prims.of_int (6))
-                                                                    (Prims.of_int (433))
+                                                                    (Prims.of_int (462))
+                                                                    (Prims.of_int (54))
+                                                                    (Prims.of_int (465))
                                                                     (Prims.of_int (59)))))
                                                                     (FStar_Tactics_Effect.lift_div_tac
                                                                     (fun
-                                                                    uu___13
+                                                                    uu___11
+                                                                    ->
+                                                                    uu___10))
+                                                                    (fun
+                                                                    uu___11
+                                                                    ->
+                                                                    (fun
+                                                                    uu___11
+                                                                    ->
+                                                                    Obj.magic
+                                                                    (FStar_Tactics_Effect.tac_bind
+                                                                    (FStar_Sealed.seal
+                                                                    (Obj.magic
+                                                                    (FStar_Range.mk_range
+                                                                    "Pulse.Checker.WithInv.fst"
+                                                                    (Prims.of_int (464))
+                                                                    (Prims.of_int (8))
+                                                                    (Prims.of_int (464))
+                                                                    (Prims.of_int (31)))))
+                                                                    (FStar_Sealed.seal
+                                                                    (Obj.magic
+                                                                    (FStar_Range.mk_range
+                                                                    "Pulse.Checker.WithInv.fst"
+                                                                    (Prims.of_int (465))
+                                                                    (Prims.of_int (6))
+                                                                    (Prims.of_int (465))
+                                                                    (Prims.of_int (59)))))
+                                                                    (FStar_Tactics_Effect.lift_div_tac
+                                                                    (fun
+                                                                    uu___12
                                                                     ->
                                                                     Pulse_Typing.T_Sub
-                                                                    (g,
-                                                                    (Pulse_Typing.wtag
-                                                                    (FStar_Pervasives_Native.Some
-                                                                    Pulse_Syntax_Base.STT_Atomic)
-                                                                    (Pulse_Syntax_Base.Tm_WithInv
-                                                                    {
-                                                                    Pulse_Syntax_Base.name1
-                                                                    = i;
-                                                                    Pulse_Syntax_Base.body6
-                                                                    = body1;
-                                                                    Pulse_Syntax_Base.returns_inv
-                                                                    =
-                                                                    FStar_Pervasives_Native.None
-                                                                    })),
+                                                                    (g, tm,
                                                                     c_out,
-                                                                    (Pulse_Syntax_Base.C_STAtomic
-                                                                    (opens,
-                                                                    obs1,
-                                                                    st1)), d,
-                                                                    (Pulse_Typing.STS_AtomicInvs
-                                                                    (g, st1,
-                                                                    add_inv,
-                                                                    opens,
-                                                                    obs1,
-                                                                    obs1, ())))))
+                                                                    c_out_opens,
+                                                                    d,
+                                                                    d_sub_c)))
                                                                     (fun
-                                                                    uu___13
+                                                                    uu___12
                                                                     ->
                                                                     (fun d1
                                                                     ->
@@ -1982,26 +1991,184 @@ let (check :
                                                                     g pre
                                                                     post_hint
                                                                     (FStar_Pervasives.Mkdtuple3
-                                                                    ((Pulse_Typing.wtag
-                                                                    (FStar_Pervasives_Native.Some
-                                                                    Pulse_Syntax_Base.STT_Atomic)
-                                                                    (Pulse_Syntax_Base.Tm_WithInv
-                                                                    {
-                                                                    Pulse_Syntax_Base.name1
-                                                                    = i;
-                                                                    Pulse_Syntax_Base.body6
-                                                                    = body1;
-                                                                    Pulse_Syntax_Base.returns_inv
-                                                                    =
-                                                                    FStar_Pervasives_Native.None
-                                                                    })),
-                                                                    c_out1,
+                                                                    (tm,
+                                                                    c_out_opens,
                                                                     d1))
                                                                     res_ppname))
-                                                                    uu___13)))
-                                                                    uu___13)))
-                                                                    uu___13)))
-                                                                    uu___12))
+                                                                    uu___12)))
+                                                                    uu___11)))
+                                                                    uu___10)))
+                                                                    uu___10))
+                                                                    | 
+                                                                    Pulse_Syntax_Base.EffectAnnotAtomic
+                                                                    uu___9 ->
+                                                                    Obj.magic
+                                                                    (FStar_Tactics_Effect.tac_bind
+                                                                    (FStar_Sealed.seal
+                                                                    (Obj.magic
+                                                                    (FStar_Range.mk_range
+                                                                    "Pulse.Checker.WithInv.fst"
+                                                                    (Prims.of_int (453))
+                                                                    (Prims.of_int (8))
+                                                                    (Prims.of_int (453))
+                                                                    (Prims.of_int (60)))))
+                                                                    (FStar_Sealed.seal
+                                                                    (Obj.magic
+                                                                    (FStar_Range.mk_range
+                                                                    "Pulse.Checker.WithInv.fst"
+                                                                    (Prims.of_int (454))
+                                                                    (Prims.of_int (8))
+                                                                    (Prims.of_int (465))
+                                                                    (Prims.of_int (59)))))
+                                                                    (Obj.magic
+                                                                    (add_remove_inverse
+                                                                    g opens i
+                                                                    () ()))
+                                                                    (fun
+                                                                    uu___10
+                                                                    ->
+                                                                    (fun tok1
+                                                                    ->
+                                                                    Obj.magic
+                                                                    (FStar_Tactics_Effect.tac_bind
+                                                                    (FStar_Sealed.seal
+                                                                    (Obj.magic
+                                                                    (FStar_Range.mk_range
+                                                                    "Pulse.Checker.WithInv.fst"
+                                                                    (Prims.of_int (456))
+                                                                    (Prims.of_int (8))
+                                                                    (Prims.of_int (462))
+                                                                    (Prims.of_int (51)))))
+                                                                    (FStar_Sealed.seal
+                                                                    (Obj.magic
+                                                                    (FStar_Range.mk_range
+                                                                    "Pulse.Checker.WithInv.fst"
+                                                                    (Prims.of_int (454))
+                                                                    (Prims.of_int (8))
+                                                                    (Prims.of_int (465))
+                                                                    (Prims.of_int (59)))))
+                                                                    (FStar_Tactics_Effect.lift_div_tac
+                                                                    (fun
+                                                                    uu___10
+                                                                    ->
+                                                                    match c_out
+                                                                    with
+                                                                    | 
+                                                                    Pulse_Syntax_Base.C_STAtomic
+                                                                    (add_inv,
+                                                                    obs, st)
+                                                                    ->
+                                                                    Prims.Mkdtuple2
+                                                                    ((Pulse_Syntax_Base.C_STAtomic
+                                                                    (opens,
+                                                                    obs, st)),
+                                                                    (Pulse_Typing.STS_AtomicInvs
+                                                                    (g, st,
+                                                                    add_inv,
+                                                                    opens,
+                                                                    obs, obs,
+                                                                    ())))
+                                                                    | 
+                                                                    Pulse_Syntax_Base.C_STGhost
+                                                                    (add_inv,
+                                                                    st) ->
+                                                                    Prims.Mkdtuple2
+                                                                    ((Pulse_Syntax_Base.C_STGhost
+                                                                    (opens,
+                                                                    st)),
+                                                                    (Pulse_Typing.STS_GhostInvs
+                                                                    (g, st,
+                                                                    add_inv,
+                                                                    opens,
+                                                                    ())))))
+                                                                    (fun
+                                                                    uu___10
+                                                                    ->
+                                                                    (fun
+                                                                    uu___10
+                                                                    ->
+                                                                    match uu___10
+                                                                    with
+                                                                    | 
+                                                                    Prims.Mkdtuple2
+                                                                    (c_out_opens,
+                                                                    d_sub_c)
+                                                                    ->
+                                                                    Obj.magic
+                                                                    (FStar_Tactics_Effect.tac_bind
+                                                                    (FStar_Sealed.seal
+                                                                    (Obj.magic
+                                                                    (FStar_Range.mk_range
+                                                                    "Pulse.Checker.WithInv.fst"
+                                                                    (Prims.of_int (462))
+                                                                    (Prims.of_int (54))
+                                                                    (Prims.of_int (465))
+                                                                    (Prims.of_int (59)))))
+                                                                    (FStar_Sealed.seal
+                                                                    (Obj.magic
+                                                                    (FStar_Range.mk_range
+                                                                    "Pulse.Checker.WithInv.fst"
+                                                                    (Prims.of_int (462))
+                                                                    (Prims.of_int (54))
+                                                                    (Prims.of_int (465))
+                                                                    (Prims.of_int (59)))))
+                                                                    (FStar_Tactics_Effect.lift_div_tac
+                                                                    (fun
+                                                                    uu___11
+                                                                    ->
+                                                                    uu___10))
+                                                                    (fun
+                                                                    uu___11
+                                                                    ->
+                                                                    (fun
+                                                                    uu___11
+                                                                    ->
+                                                                    Obj.magic
+                                                                    (FStar_Tactics_Effect.tac_bind
+                                                                    (FStar_Sealed.seal
+                                                                    (Obj.magic
+                                                                    (FStar_Range.mk_range
+                                                                    "Pulse.Checker.WithInv.fst"
+                                                                    (Prims.of_int (464))
+                                                                    (Prims.of_int (8))
+                                                                    (Prims.of_int (464))
+                                                                    (Prims.of_int (31)))))
+                                                                    (FStar_Sealed.seal
+                                                                    (Obj.magic
+                                                                    (FStar_Range.mk_range
+                                                                    "Pulse.Checker.WithInv.fst"
+                                                                    (Prims.of_int (465))
+                                                                    (Prims.of_int (6))
+                                                                    (Prims.of_int (465))
+                                                                    (Prims.of_int (59)))))
+                                                                    (FStar_Tactics_Effect.lift_div_tac
+                                                                    (fun
+                                                                    uu___12
+                                                                    ->
+                                                                    Pulse_Typing.T_Sub
+                                                                    (g, tm,
+                                                                    c_out,
+                                                                    c_out_opens,
+                                                                    d,
+                                                                    d_sub_c)))
+                                                                    (fun
+                                                                    uu___12
+                                                                    ->
+                                                                    (fun d1
+                                                                    ->
+                                                                    Obj.magic
+                                                                    (Pulse_Checker_Base.checker_result_for_st_typing
+                                                                    g pre
+                                                                    post_hint
+                                                                    (FStar_Pervasives.Mkdtuple3
+                                                                    (tm,
+                                                                    c_out_opens,
+                                                                    d1))
+                                                                    res_ppname))
+                                                                    uu___12)))
+                                                                    uu___11)))
+                                                                    uu___10)))
+                                                                    uu___10))
                                                                     | 
                                                                     Pulse_Syntax_Base.EffectAnnotSTT
                                                                     ->
@@ -2011,37 +2178,23 @@ let (check :
                                                                     (Obj.magic
                                                                     (FStar_Range.mk_range
                                                                     "Pulse.Checker.WithInv.fst"
-                                                                    (Prims.of_int (436))
+                                                                    (Prims.of_int (468))
                                                                     (Prims.of_int (14))
-                                                                    (Prims.of_int (436))
+                                                                    (Prims.of_int (468))
                                                                     (Prims.of_int (57)))))
                                                                     (FStar_Sealed.seal
                                                                     (Obj.magic
                                                                     (FStar_Range.mk_range
                                                                     "Pulse.Checker.WithInv.fst"
-                                                                    (Prims.of_int (437))
+                                                                    (Prims.of_int (469))
                                                                     (Prims.of_int (6))
-                                                                    (Prims.of_int (437))
+                                                                    (Prims.of_int (469))
                                                                     (Prims.of_int (59)))))
                                                                     (FStar_Tactics_Effect.lift_div_tac
                                                                     (fun
-                                                                    uu___11
-                                                                    ->
+                                                                    uu___9 ->
                                                                     Pulse_Typing.T_Lift
-                                                                    (g,
-                                                                    (Pulse_Typing.wtag
-                                                                    (FStar_Pervasives_Native.Some
-                                                                    Pulse_Syntax_Base.STT_Atomic)
-                                                                    (Pulse_Syntax_Base.Tm_WithInv
-                                                                    {
-                                                                    Pulse_Syntax_Base.name1
-                                                                    = i;
-                                                                    Pulse_Syntax_Base.body6
-                                                                    = body1;
-                                                                    Pulse_Syntax_Base.returns_inv
-                                                                    =
-                                                                    FStar_Pervasives_Native.None
-                                                                    })),
+                                                                    (g, tm,
                                                                     c_out,
                                                                     (Pulse_Syntax_Base.C_ST
                                                                     (Pulse_Syntax_Base.st_comp_of_comp
@@ -2051,8 +2204,7 @@ let (check :
                                                                     (g,
                                                                     c_out)))))
                                                                     (fun
-                                                                    uu___11
-                                                                    ->
+                                                                    uu___9 ->
                                                                     (fun d1
                                                                     ->
                                                                     Obj.magic
@@ -2060,49 +2212,36 @@ let (check :
                                                                     g pre
                                                                     post_hint
                                                                     (FStar_Pervasives.Mkdtuple3
-                                                                    ((Pulse_Typing.wtag
-                                                                    (FStar_Pervasives_Native.Some
-                                                                    Pulse_Syntax_Base.STT_Atomic)
-                                                                    (Pulse_Syntax_Base.Tm_WithInv
-                                                                    {
-                                                                    Pulse_Syntax_Base.name1
-                                                                    = i;
-                                                                    Pulse_Syntax_Base.body6
-                                                                    = body1;
-                                                                    Pulse_Syntax_Base.returns_inv
-                                                                    =
-                                                                    FStar_Pervasives_Native.None
-                                                                    })),
+                                                                    (tm,
                                                                     (Pulse_Syntax_Base.C_ST
                                                                     (Pulse_Syntax_Base.st_comp_of_comp
                                                                     c_out)),
                                                                     d1))
                                                                     res_ppname))
-                                                                    uu___11)))
-                                                                    uu___11)))
-                                                                    uu___11)))
-                                                                    uu___11)))
-                                                                    uu___10)))
                                                                     uu___9)))
                                                                     uu___9)))
                                                                     uu___9)))
                                                                     uu___9)))
                                                                     uu___9)))
                                                                     uu___8)))
+                                                                    uu___8)))
+                                                                    uu___8)))
+                                                                    uu___8)))
+                                                                    uu___8)))
                                                                     uu___7)))
-                                                                    uu___7)))
-                                                                    uu___5)))
-                                                                    uu___4)))
-                                                                    uu___4)))
-                                                                    uu___4)))
-                                                                    uu___4)))
-                                                                    uu___4)))
-                                                                    uu___4)))
-                                                                    uu___4)))
+                                                                    uu___6)))
+                                                                    uu___6)))
                                                                     uu___4)))
                                                                     uu___3)))
+                                                                    uu___3)))
+                                                                    uu___3)))
+                                                                    uu___3)))
+                                                                    uu___3)))
+                                                                    uu___3)))
+                                                                    uu___3)))
+                                                                    uu___3)))
                                                                     uu___2)))
-                                                                    uu___2)))
-                                                                uu___2)))
-                                                     uu___2))) uu___1)))
-                       uu___)
+                                                                    uu___1)))
+                                                                    uu___1)))
+                                                            uu___1))) uu___1)))
+                                      uu___1))) uu___)
